cogent/examples/wa_connect/WordArray_CorresProof_Asm.thy
@@ -526,186 +526,104 @@ lemma lit_type_ex:
   apply (induct l; clarsimp)+
   done
 
-lemma 
+lemma val_wa_foldnb_bod_rename_monoexpr_correct:
   "\<lbrakk>val.proc_env_matches \<xi>\<^sub>m \<Xi>'; proc_ctx_wellformed \<Xi>'; 
-    val_wa_foldnb_bod \<xi>\<^sub>m xs frm to (Fun (val.rename_expr rename' (val.monoexpr (specialise ts f))) [])
-         acc obsv res;
-\<forall>i<length xs. \<exists>v. xs ! i = VPrim (LU32 v);
-    \<Xi>, [], [option.Some Generated_TypeProof.abbreviatedType1] \<turnstile> App (Fun (val.rename_expr rename 
-      (val.monoexpr (specialise ts f))) []) (Var 0) : TPrim (Num U32)
-    \<rbrakk>
-       \<Longrightarrow> val_wa_foldnb_bod \<xi>\<^sub>p xs frm to (Fun f ts) acc obsv (VPrim (LU32 r))"
-  oops
-
-lemma val_wa_foldnb_0_mono_helper1:
-  "\<lbrakk>val.proc_env_matches \<xi>m1 \<Xi>; proc_ctx_wellformed \<Xi>; \<forall>i<length xs. \<exists>v. xs ! i = VPrim (LU32 v);
-    \<Xi>, [], [option.Some Generated_TypeProof.abbreviatedType1] \<turnstile> App (Fun (val.rename_expr rename 
-      (val.monoexpr (specialise ts f))) []) (Var 0) : TPrim (Num U32);
-    val_wa_foldnb_bod \<xi>m xs frm to (Fun (val.rename_expr rename (val.monoexpr (specialise ts f))) [])
-         (VPrim (LU32 acc)) VUnit (VPrim (LU32 r))\<rbrakk>
-       \<Longrightarrow> val_wa_foldnb_bod \<xi>p xs frm to (Fun f ts) (VPrim (LU32 acc)) VUnit (VPrim (LU32 r))"
+    value_sem.rename_mono_prog wa_abs_typing_v rename' \<Xi>' \<xi>\<^sub>m \<xi>\<^sub>p;
+    val_wa_foldnb_bod \<xi>\<^sub>m xs frm to (vvalfun_to_exprfun (val.rename_val rename' (val.monoval f))) 
+      (val.rename_val rename' (val.monoval acc )) (val.rename_val rename' (val.monoval obsv)) r;
+    is_vval_fun (val.rename_val rename' (val.monoval f)); wa_abs_typing_v (VWA t xs) ''WordArray'' [t]; 
+    val.vval_typing \<Xi>' (val.rename_val rename' (val.monoval acc )) u;
+    val.vval_typing \<Xi>' (val.rename_val rename' (val.monoval obsv)) v;
+    \<Xi>', [], [option.Some (TRecord [(a0, t, Present), (a1, u, Present), (a2, v, Present)] Unboxed)] \<turnstile>
+      App (vvalfun_to_exprfun (val.rename_val rename' (val.monoval f))) (Var 0) : u; 
+    distinct [a0, a1, a2]\<rbrakk>
+       \<Longrightarrow> is_vval_fun f \<and> (\<exists>r'. r = val.rename_val rename' (val.monoval r') \<and>
+         val_wa_foldnb_bod \<xi>\<^sub>p xs frm to (vvalfun_to_exprfun f) acc obsv r')"
+  apply (rule conjI)
+   apply (case_tac f; clarsimp)
   apply (induct to arbitrary: r)
    apply (erule val_wa_foldnb_bod.elims; clarsimp)
    apply (subst val_wa_foldnb_bod.simps; clarsimp)
-  apply clarsimp
   apply (case_tac "length xs < Suc to")
-   apply (erule_tac x = r in meta_allE)
    apply (drule val_wa_foldnb_bod_back_step'; simp)
    apply (drule val_wa_foldnb_bod_to_geq_lenD)
     apply linarith
-   apply (rule val_wa_foldnb_bod_to_geq_len; simp)
-  apply (clarsimp simp: not_less)
+   apply (drule_tac x = r in meta_spec)
+   apply clarsimp
+   apply (erule meta_impE)
+    apply (rule val_wa_foldnb_bod_to_geq_len; simp?)
+   apply clarsimp
+   apply (rule_tac x = r' in exI; clarsimp)
+   apply (rule val_wa_foldnb_bod_to_geq_len; simp?)
+   apply (drule_tac to = to in val_wa_foldnb_bod_to_geq_lenD; simp?)
   apply (case_tac "frm \<ge> to")
+  apply (clarsimp simp: not_less not_le)
    apply (erule val_wa_foldnb_bod.elims; clarsimp split: if_splits)
     apply (erule val_wa_foldnb_bod.elims; clarsimp)
     apply (subst val_wa_foldnb_bod.simps; clarsimp)
     apply (subst val_wa_foldnb_bod.simps; clarsimp)
-    apply (drule_tac \<gamma> = "[VRecord [xs ! frm, VPrim (LU32 acc), VUnit]]" and
-      \<Gamma> = "[option.Some abbreviatedType1]" and
-      e = "App (Fun f ts) (Var 0)" and
-      v' = "VPrim (LU32 r)" and
-      \<tau>  = "TPrim (Num U32)" in val.rename_monoexpr_correct(1)
-      [OF _ val_proc_env_matches_\<xi>m_\<Xi> value_sem_rename_mono_prog_rename_\<Xi>_\<xi>m_\<xi>p]; clarsimp?)
-      apply (clarsimp simp: abbreviatedType1_def)
-      apply (clarsimp simp: val.matches_Cons[where xs = "[]" and ys = "[]", simplified])
-      apply (clarsimp simp: val.matches_def)
-      apply (rule val.v_t_record; simp?)
-      apply (rule val.v_t_r_cons1; clarsimp?)
-       apply (erule_tac x = frm in allE; clarsimp)
-       apply (rule val.v_t_prim'; clarsimp)
-      apply (rule val.v_t_r_cons1; clarsimp?)
-       apply (rule val.v_t_prim'; clarsimp)
-      apply (rule val.v_t_r_cons1; clarsimp?)
-       apply (rule val.v_t_unit)
-      apply (rule val.v_t_r_empty)
-     apply (erule_tac x = frm in allE; clarsimp)
-    apply (case_tac v; clarsimp)
+    apply (frule_tac \<gamma> = "[VRecord [xs ! frm, acc, obsv]]" and
+      ?\<Gamma> = "[option.Some (TRecord [(a0, t, Present), (a1, u, Present), (a2, v, Present)] Unboxed)]" and
+      e = "App (vvalfun_to_exprfun f) (Var 0)" and
+      v' = resa and
+      \<tau> = u in val.rename_monoexpr_correct(1); simp?)
+       apply (clarsimp simp: val.matches_Cons[where xs = "[]" and ys = "[]", simplified])
+       apply (clarsimp simp: val.matches_def)
+       apply (rule val.v_t_record; simp?)
+       apply (rule val.v_t_r_cons1; clarsimp?)
+        apply (clarsimp simp: wa_abs_typing_v_def)
+        apply (case_tac t; clarsimp)
+        apply (case_tac x5; clarsimp)
+        apply (erule_tac x = frm in allE; clarsimp)
+        apply (rule val.v_t_prim'; clarsimp)
+       apply (rule val.v_t_r_cons1; clarsimp?)
+       apply (rule val.v_t_r_cons1; clarsimp?)
+       apply (rule val.v_t_r_empty)
+      apply (clarsimp simp: wa_abs_typing_v_def)
+      apply (case_tac t; clarsimp)
+      apply (case_tac x5; clarsimp)
+      apply (erule_tac x = frm in allE; clarsimp)
+      apply (case_tac f; clarsimp)
+     apply (case_tac f; clarsimp)
+    apply clarsimp
+    apply (rule_tac x = va in exI; clarsimp)
+   apply (clarsimp simp: not_le not_less)
    apply (subst val_wa_foldnb_bod.simps; clarsimp)
-  apply (clarsimp simp: not_le)
-  apply (frule_tac x = to in spec)
-  apply (erule impE, simp)
-  apply (erule exE)
+  apply (clarsimp simp: not_le not_less)
   apply (drule val_wa_foldnb_bod_back_step; simp?)
   apply clarsimp
-  apply (subgoal_tac "\<exists>y. r' = VPrim (LU32 y)", clarsimp)
-   apply (erule_tac x = y in meta_allE)
-   apply clarsimp
-   apply (drule_tac \<gamma> = "[VRecord [VPrim (LU32 v), VPrim (LU32 y), VUnit]]" and
-      \<Gamma> = "[option.Some abbreviatedType1]" and
-      e = "App (Fun f ts) (Var 0)" and
-      v' = "VPrim (LU32 r)" and
-      \<tau>  = "TPrim (Num U32)" in val.rename_monoexpr_correct(1)
-      [OF _ val_proc_env_matches_\<xi>m_\<Xi> value_sem_rename_mono_prog_rename_\<Xi>_\<xi>m_\<xi>p]; clarsimp?)
-    apply (clarsimp simp: abbreviatedType1_def)
-    apply (clarsimp simp: val.matches_Cons[where xs = "[]" and ys = "[]", simplified])
-    apply (clarsimp simp: val.matches_def)
-    apply (rule val.v_t_record; simp?)
-    apply (rule val.v_t_r_cons1; clarsimp?)
-     apply (rule val.v_t_prim'; clarsimp)
-    apply (rule val.v_t_r_cons1; clarsimp?)
-     apply (rule val.v_t_prim'; clarsimp)
-    apply (rule val.v_t_r_cons1; clarsimp?)
-     apply (rule val.v_t_unit)
-    apply (rule val.v_t_r_empty)
-   apply (case_tac va; clarsimp)
-   apply (drule_tac r' = "VPrim (LU32 r)" in val_wa_foldnb_bod_step; simp)
-  apply (insert val_proc_env_matches_\<xi>m_\<Xi>)
-  apply (clarsimp simp: abbreviatedType1_def)
-  apply (drule val_wa_foldnb_bod_preservation; simp?)
-     apply (clarsimp simp: wa_abs_typing_v_def)
-     apply (erule_tac x = i in allE; clarsimp)
-     apply (rule val.v_t_prim'; clarsimp)
-    apply (rule val.v_t_unit)
-   apply clarsimp
-  apply (erule v_t_prim_tE)
-  apply (drule lit_type_ex[OF sym])
+  apply (drule_tac x = r' in meta_spec)
+  apply clarsimp
+  apply (frule_tac \<gamma> = "[VRecord [xs ! to, r'a, obsv]]" and
+      ?\<Gamma> = "[option.Some (TRecord [(a0, t, Present), (a1, u, Present), (a2, v, Present)] Unboxed)]" and
+      e = "App (vvalfun_to_exprfun f) (Var 0)" and
+      v' = r and
+      \<tau> = u in val.rename_monoexpr_correct(1); simp?)
+     apply (clarsimp simp: val.matches_Cons[where xs = "[]" and ys = "[]", simplified])
+     apply (clarsimp simp: val.matches_def)
+     apply (rule val.v_t_record; simp?)
+     apply (rule val.v_t_r_cons1; clarsimp?)
+      apply (clarsimp simp: wa_abs_typing_v_def)
+      apply (case_tac t; clarsimp)
+      apply (case_tac x5; clarsimp)
+      apply (erule_tac x = to in allE; clarsimp)
+      apply (rule val.v_t_prim'; clarsimp)
+     apply (rule val.v_t_r_cons1; clarsimp?)
+      apply (drule val_wa_foldnb_bod_preservation; simp?)
+     apply (rule val.v_t_r_cons1; clarsimp?)
+     apply (rule val.v_t_r_empty)
+    apply (clarsimp simp: wa_abs_typing_v_def)
+    apply (case_tac t; clarsimp)
+    apply (case_tac x5; clarsimp)
+    apply (erule_tac x = to in allE; clarsimp)
+    apply (case_tac f; clarsimp)
+   apply (case_tac f; clarsimp)
+  apply clarsimp
+  apply (drule_tac \<xi>\<^sub>v = \<xi>\<^sub>p in val_wa_foldnb_bod_step; simp?)
+  apply (rule_tac x = va in exI)
   apply clarsimp
   done
 
-lemma val_wa_foldnb_0_mono_helper2:
-  "\<lbrakk>val.proc_env_matches \<xi>m1 \<Xi>; proc_ctx_wellformed \<Xi>; \<forall>i<length xs. \<exists>v. xs ! i = VPrim (LU32 v);
-    \<Xi>, [], [option.Some Generated_TypeProof.abbreviatedType1] \<turnstile> App (AFun (rename (f, ts)) []) 
-      (Var 0) : TPrim (Num U32);
-    val_wa_foldnb_bod \<xi>m xs frm to (AFun (rename (f, ts)) [])
-         (VPrim (LU32 acc)) VUnit (VPrim (LU32 r))\<rbrakk>
-       \<Longrightarrow> val_wa_foldnb_bod \<xi>p xs frm to (AFun f ts) (VPrim (LU32 acc)) VUnit (VPrim (LU32 r))"
-  apply (induct to arbitrary: r)
-   apply (erule val_wa_foldnb_bod.elims; clarsimp)
-   apply (subst val_wa_foldnb_bod.simps; clarsimp)
-  apply clarsimp
-  apply (case_tac "length xs < Suc to")
-   apply (erule_tac x = r in meta_allE)
-   apply (drule val_wa_foldnb_bod_back_step'; simp)
-   apply (drule val_wa_foldnb_bod_to_geq_lenD)
-    apply linarith
-   apply (rule val_wa_foldnb_bod_to_geq_len; simp)
-  apply (clarsimp simp: not_less)
-  apply (case_tac "frm \<ge> to")
-   apply (erule val_wa_foldnb_bod.elims; clarsimp split: if_splits)
-    apply (erule val_wa_foldnb_bod.elims; clarsimp)
-    apply (subst val_wa_foldnb_bod.simps; clarsimp)
-    apply (subst val_wa_foldnb_bod.simps; clarsimp)
-    apply (drule_tac \<gamma> = "[VRecord [xs ! frm, VPrim (LU32 acc), VUnit]]" and
-      \<Gamma> = "[option.Some abbreviatedType1]" and
-      e = "App (AFun f ts) (Var 0)" and
-      v' = "VPrim (LU32 r)" and
-      \<tau>  = "TPrim (Num U32)" in val.rename_monoexpr_correct(1)
-      [OF _ val_proc_env_matches_\<xi>m_\<Xi> value_sem_rename_mono_prog_rename_\<Xi>_\<xi>m_\<xi>p]; clarsimp?)
-      apply (clarsimp simp: abbreviatedType1_def)
-      apply (clarsimp simp: val.matches_Cons[where xs = "[]" and ys = "[]", simplified])
-      apply (clarsimp simp: val.matches_def)
-      apply (rule val.v_t_record; simp?)
-      apply (rule val.v_t_r_cons1; clarsimp?)
-       apply (erule_tac x = frm in allE; clarsimp)
-       apply (rule val.v_t_prim'; clarsimp)
-      apply (rule val.v_t_r_cons1; clarsimp?)
-       apply (rule val.v_t_prim'; clarsimp)
-      apply (rule val.v_t_r_cons1; clarsimp?)
-       apply (rule val.v_t_unit)
-      apply (rule val.v_t_r_empty)
-     apply (erule_tac x = frm in allE; clarsimp)
-    apply (case_tac v; clarsimp)
-   apply (subst val_wa_foldnb_bod.simps; clarsimp)
-  apply (clarsimp simp: not_le)
-  apply (frule_tac x = to in spec)
-  apply (erule impE, simp)
-  apply (erule exE)
-  apply (drule val_wa_foldnb_bod_back_step; simp?)
-  apply clarsimp
-  apply (subgoal_tac "\<exists>y. r' = VPrim (LU32 y)", clarsimp)
-   apply (erule_tac x = y in meta_allE)
-   apply clarsimp
-   apply (drule_tac \<gamma> = "[VRecord [VPrim (LU32 v), VPrim (LU32 y), VUnit]]" and
-      \<Gamma> = "[option.Some abbreviatedType1]" and
-      e = "App (AFun f ts) (Var 0)" and
-      v' = "VPrim (LU32 r)" and
-      \<tau>  = "TPrim (Num U32)" in val.rename_monoexpr_correct(1)
-      [OF _ val_proc_env_matches_\<xi>m_\<Xi> value_sem_rename_mono_prog_rename_\<Xi>_\<xi>m_\<xi>p]; clarsimp?)
-    apply (clarsimp simp: abbreviatedType1_def)
-    apply (clarsimp simp: val.matches_Cons[where xs = "[]" and ys = "[]", simplified])
-    apply (clarsimp simp: val.matches_def)
-    apply (rule val.v_t_record; simp?)
-    apply (rule val.v_t_r_cons1; clarsimp?)
-     apply (rule val.v_t_prim'; clarsimp)
-    apply (rule val.v_t_r_cons1; clarsimp?)
-     apply (rule val.v_t_prim'; clarsimp)
-    apply (rule val.v_t_r_cons1; clarsimp?)
-     apply (rule val.v_t_unit)
-    apply (rule val.v_t_r_empty)
-   apply (case_tac va; clarsimp)
-   apply (drule_tac r' = "VPrim (LU32 r)" in val_wa_foldnb_bod_step; simp)
-  apply (insert val_proc_env_matches_\<xi>m_\<Xi>)
-  apply (clarsimp simp: abbreviatedType1_def)
-  apply (drule val_wa_foldnb_bod_preservation; simp?)
-     apply (clarsimp simp: wa_abs_typing_v_def)
-     apply (erule_tac x = i in allE; clarsimp)
-     apply (rule val.v_t_prim'; clarsimp)
-    apply (rule val.v_t_unit)
-   apply clarsimp
-  apply (erule v_t_prim_tE)
-  apply (drule lit_type_ex[OF sym])
-  apply clarsimp
-  done
 
 lemma value_sem_rename_mono_prog_rename_\<Xi>_\<xi>m1_\<xi>p1: 
   "value_sem.rename_mono_prog wa_abs_typing_v rename \<Xi> \<xi>m1 \<xi>p1"
@@ -734,18 +652,23 @@ lemma value_sem_rename_mono_prog_rename_\<Xi>_\<xi>m1_\<xi>p1:
   apply (subst (asm) assoc_lookup.simps)+
   apply (clarsimp split: if_split_asm simp: val_wa_foldnb_0_def val_wa_foldnb_0p_def)
   apply (case_tac v; clarsimp)
+  apply (clarsimp simp: abbreviatedType1_def)
+  thm val_wa_foldnb_bod_rename_monoexpr_correct
+  apply (drule_tac xs = xs and frm = "unat frm" and to = "unat to" and acc = zd and obsv = ze and
+      r = "(VPrim (LU32 r))" and \<xi>\<^sub>p = \<xi>p in 
+      val_wa_foldnb_bod_rename_monoexpr_correct[OF val_proc_env_matches_\<xi>m_\<Xi>] ; simp?)
+       apply (rule value_sem_rename_mono_prog_rename_\<Xi>_\<xi>m_\<xi>p)
+      apply (clarsimp simp: wa_abs_typing_v_def)
+      apply (erule_tac x = i in allE; clarsimp)
+     apply (rule val.v_t_prim'; clarsimp)
+    apply (rule val.v_t_unit)
+   apply clarsimp
+  apply clarsimp
+  apply (rule_tac x = r' in exI; clarsimp)
   apply (case_tac z; clarsimp)
   apply (case_tac za; clarsimp)
-  apply (case_tac zb; clarsimp)
-  apply (case_tac zd; clarsimp)
-  apply (case_tac ze; clarsimp)
-  apply (rule_tac x = "VPrim (LU32 r)" in exI)
-  apply clarsimp
-  apply (case_tac zc; clarsimp)
-   apply (clarsimp simp: val_wa_foldnb_0_mono_helper1)
-  apply (clarsimp simp: val_wa_foldnb_0_mono_helper2)
+  apply(case_tac zb; clarsimp)
   done
-
 
 lemma val_proc_env_matches_\<xi>m1_\<Xi>:
   "val.proc_env_matches \<xi>m1 \<Xi>"
@@ -1339,84 +1262,6 @@ lemma proc_env_u_v_matches_\<xi>1_\<xi>m1_\<Xi>:
    apply (drule wa_put2_upd_val; simp)
   apply (clarsimp simp: wordarray_fold_no_break_upd_val)
   done
-
-(*
-
-
-lemma 
-  "\<lbrakk>val_wa_foldnb_bod xs frm (Suc to) f acc obsv r; frm < Suc to\<rbrakk>
-    \<Longrightarrow> \<exists>acc'. val_wa_foldnb_bod xs to (Suc to) f acc' obsv r"
-  apply (induct rule: val_wa_foldnb_bod.induct[where ?a0.0 = xs and
-                                                       ?a1.0 = frm and
-                                                       ?a2.0 = to and
-                                                       ?a3.0 = f and
-                                                       ?a4.0 = acc and
-                                                       ?a5.0 = obsv and
-                                                       ?a6.0 = r]; clarsimp)
-  apply (case_tac "frm < length xs")
-   apply (case_tac "frm < to")
-    apply (erule val_wa_foldnb_bod.elims; clarsimp)
-   apply clarsimp
-   apply (rule_tac x = acc in exI)
-   apply (erule val_wa_foldnb_bod.elims; clarsimp)+
-   apply (subst val_wa_foldnb_bod.simps; clarsimp)+
-   apply (rule_tac x = v in exI)
-   apply clarsimp
-   apply (subgoal_tac "frma = to")
-    apply clarsimp
-   apply linarith
-  apply (rule_tac x = res in exI)
-  apply (subst val_wa_foldnb_bod.simps; clarsimp)
-  done
-lemma 
-  "\<lbrakk>val_wa_foldnb_bod xs frm to f (VPrim (LU32 acc)) VUnit r; 
-    \<forall>i<length xs. \<exists>v. xs ! i = VPrim (LU32 v);
-    \<Xi>, [], [option.Some abbreviatedType1] \<turnstile> App f (Var 0) : TPrim (Num U32)\<rbrakk>
-    \<Longrightarrow> \<exists>x. r = VPrim (LU32 x)"
-  apply (induct to arbitrary: r)
-   apply (erule val_wa_foldnb_bod.elims; clarsimp)
-  apply (case_tac "length xs < Suc to")
-   apply (drule val_wa_foldnb_bod_back_step'; simp)
-  apply (case_tac "to \<le> frm")
-   apply (erule val_wa_foldnb_bod.elims; clarsimp split: if_splits)
-   apply (erule val_wa_foldnb_bod.elims; clarsimp)
-   apply (insert proc_ctx_wellformed_\<Xi> val_proc_env_matches_\<xi>m_\<Xi>)
-   apply (drule val.preservation(1)[of "[]" "[]" _ _ _  \<xi>m, simplified]; simp?)
-    apply (clarsimp simp: abbreviatedType1_def)
-    apply (clarsimp simp: val.matches_Cons[where xs = "[]" and ys = "[]", simplified])
-    apply (clarsimp simp: val.matches_def)
-    apply (rule val.v_t_record; simp?)
-    apply (rule val.v_t_r_cons1; clarsimp?)
-     apply (rule val.v_t_prim'; clarsimp)
-    apply (rule val.v_t_r_cons1; clarsimp?)
-     apply (rule val.v_t_prim'; clarsimp)
-    apply (rule val.v_t_r_cons1; clarsimp?)
-     apply (rule val.v_t_unit)
-    apply (rule val.v_t_r_empty)
-   apply (erule v_t_prim_tE; clarsimp simp: lit_type_ex)
-  apply (clarsimp simp: not_less not_le)
-  apply (erule_tac x = to in allE; clarsimp)
-  apply (drule val_wa_foldnb_bod_back_step; simp?)
-  apply clarsimp
-  apply (drule_tac x = r' in meta_spec)
-  apply clarsimp
-  apply (insert proc_ctx_wellformed_\<Xi> val_proc_env_matches_\<xi>m_\<Xi>)
-  apply (drule val.preservation(1)[of "[]" "[]" _ _ _  \<xi>m, simplified]; simp?)
-   apply (clarsimp simp: abbreviatedType1_def)
-   apply (clarsimp simp: val.matches_Cons[where xs = "[]" and ys = "[]", simplified])
-   apply (clarsimp simp: val.matches_def)
-   apply (rule val.v_t_record; simp?)
-   apply (rule val.v_t_r_cons1; clarsimp?)
-    apply (rule val.v_t_prim'; clarsimp)
-   apply (rule val.v_t_r_cons1; clarsimp?)
-    apply (rule val.v_t_prim'; clarsimp)
-   apply (rule val.v_t_r_cons1; clarsimp?)
-    apply (rule val.v_t_unit)
-   apply (rule val.v_t_r_empty)
-  apply (erule v_t_prim_tE; clarsimp simp: lit_type_ex)
-  done
-
-*)
 
 end (* of context *)
 
